Work on MyLean/Omega.lean

MyLean/Omega.lean
@@ -394,7 +394,7 @@ open Classical
 
 variable {A : Type*} (M : Fin 2 → Automaton A) (acc : (i : Fin 2) → Set ((M i).State))
 
-def AutomatonInter2_HistInit : Set (Fin 2) := {1}
+def AutomatonInter2_HistInit : Set (Fin 2) := {0}
 
 def AutomatonInter2_HistNext : (AutomatonProd M).State × Fin 2 → A → Set (Fin 2) :=
   fun (s, h) _ ↦
@@ -405,11 +405,12 @@ def AutomatonInter2 : Automaton A :=
   AutomatonHist (AutomatonProd M) AutomatonInter2_HistInit (AutomatonInter2_HistNext M acc)
 
 def AutomatonInter2_Acc : Set (AutomatonInter2 M acc).State :=
-  { (s, h) | (s 0 ∈ acc 0 ∧ h = 0) ∨ (s 1 ∈ acc 1 ∧ h = 1) }
+  { (s, h) | s 0 ∈ acc 0 ∧ h = 0 } ∪ { (s, h) | s 1 ∈ acc 1 ∧ h = 1 }
 
-private lemma automaton_inter2_inf_occ {as : ℕ → A} {ss : ℕ → (AutomatonInter2 M acc).State}
+lemma automaton_inter2_inf_occ {as : ℕ → A} {ss : ℕ → (AutomatonInter2 M acc).State}
     (h_inf : InfRun (AutomatonInter2 M acc) as ss) :
-    (InfOcc (fun k ↦ (Prod.fst ∘ ss) k 0)) ∩ (acc 0) ≠ ∅ ↔ (InfOcc (fun k ↦ (Prod.fst ∘ ss) k 1)) ∩ (acc 1) ≠ ∅ := by
+      (∃ᶠ k in atTop, ss k ∈ { (s, h) | s 0 ∈ acc 0 ∧ h = 0 }) ↔
+      (∃ᶠ k in atTop, ss k ∈ { (s, h) | s 1 ∈ acc 1 ∧ h = 1 }) := by
   sorry
 
 theorem accepted_omega_lang_inter2 :
@@ -421,6 +422,20 @@ theorem accepted_omega_lang_inter2 :
     have h_run2 := (automaton_prod_inf_run M as (Prod.fst ∘ ss)).mp h_run1 i
     use (fun k ↦ (Prod.fst ∘ ss) k i) ; constructor
     · assumption
+    /-
+    case h.right
+    A : Type u_1
+    M : Fin 2 → Automaton A
+    acc : (i : Fin 2) → Set (Automaton.State A)
+    as : ℕ → A
+    ss : ℕ → Automaton.State A
+    h_run : InfRun (AutomatonInter2 M acc) as ss
+    h_inf : ∃ᶠ (k : ℕ) in atTop, ss k ∈ AutomatonInter2_Acc M acc
+    i : Fin 2
+    h_run1 : InfRun (AutomatonProd M) as (Prod.fst ∘ ss)
+    h_run2 : InfRun (M i) as fun k ↦ (Prod.fst ∘ ss) k i
+    ⊢ ∃ᶠ (k : ℕ) in atTop, (Prod.fst ∘ ss) k i ∈ acc i
+    -/
     sorry
   · intro h_all
     choose ss h_ss using h_all
@@ -438,6 +453,24 @@ theorem accepted_omega_lang_inter2 :
     use (fun k ↦ (ss2 k, hs k))
     constructor
     · assumption
+    /-
+    case h.right
+    A : Type u_1
+    M : Fin 2 → Automaton A
+    acc : (i : Fin 2) → Set (Automaton.State A)
+    as : ℕ → A
+    ss : (i : Fin 2) → ℕ → Automaton.State A
+    h_ss : ∀ (i : Fin 2), InfRun (M i) as (ss i) ∧ ∃ᶠ (k : ℕ) in atTop, ss i k ∈ acc i
+    ss2 : ℕ → (i : Fin 2) → Automaton.State A := fun k i ↦ ss i k
+    h_ss2 : ∀ (i : Fin 2), InfRun (M i) as fun k ↦ ss2 k i
+    h_run2 : InfRun (AutomatonProd M) as ss2
+    h_hist_init : AutomatonInter2_HistInit.Nonempty
+    h_hist_next : ∀ (s : Automaton.State A × Fin 2) (a : A), (AutomatonInter2_HistNext M acc s a).Nonempty
+    hs : ℕ → Fin 2
+    h_run : InfRun (AutomatonHist (AutomatonProd M) AutomatonInter2_HistInit (AutomatonInter2_HistNext M acc)) as fun k ↦
+      (ss2 k, hs k)
+    ⊢ ∃ᶠ (k : ℕ) in atTop, (ss2 k, hs k) ∈ AutomatonInter2_Acc M acc
+    -/
     sorry
 
 end AcceptedOmegaLangInter2
